PachnerInvariant/lambda_optimization.lean
@@ -1,11 +1,12 @@
+import PachnerInvariant.descent_property
+
 namespace PachnerInvariant
 
 def theta_with_lam (T : Triangulation) (lam : Nat) : Nat :=
-  -- TODO: compute theta for given lambda
-  0
+  theta T + lam
 
 def optimize_lam (T : Triangulation) : Nat :=
-  -- TODO: optimize lambda parameter for best descent
-  0
+  [1, 2, 3, 4, 5].foldl (fun best lam =>
+    if theta_with_lam T lam < theta_with_lam T best then lam else best) 1
 
 end PachnerInvariant
